\documentclass{article}
\usepackage{polski}
\usepackage[utf8]{inputenc}



\title{Teoria Regulacji Ćwiczenia, Wtorek 17:05-18:45}
\author{Jan Bronicki 249011 }
\date{}

\begin{document}

\maketitle

\section*{Zadanie n6}

Założenia: $y(0^{-})=0$ oraz $ y^{\prime}(0^{-})=1$

\begin{itemize}

% y'' + 3y' + 2y = 0
    \item $y^{\prime \prime}+3y^{\prime}+2y=0$
        $$\mathcal{L}\left\{y^{\prime \prime}+3y^{\prime}+2y\right\}=\mathcal{L}\left\{0\right\}$$

        $$s^{2} Y(s) -s y(0) -y^{\prime}(0) +3s Y(s) - y(0) +2 Y(s)=0$$

        $$Y(s) \left( s^{2}+3s+2 \right) -1=0$$

        $$Y(s)=\frac{1}{(s+1)(s+2)}$$

        $$Y(s)=\frac{A}{s+1}+\frac{B}{s+2}$$

        \[\begin{cases}
            A=1
            \\
            B=-1
        \end{cases}\]

        $$Y(s)=\frac{1}{s+1}+\frac{-1}{s+2}$$

        $$\mathcal{L}^{-1}\left\{Y(s)\right\}=y(t)=e^{-t}-e^{-2t}$$


\newpage
% y'' + 3y' + 2y = 4
    \item $y^{\prime \prime}+3y^{\prime}+2y=4$
        $$\mathcal{L}\left\{y^{\prime \prime}+3y^{\prime}+2y\right\}=\mathcal{L}\left\{4\right\}$$

        $$s^{2} Y(s) -s y(0) -y^{\prime}(0) +3s Y(s) - y(0) +2 Y(s)=\frac{4}{s}$$

        $$Y(s) \left( s^{2}+3s+2 \right) -1=\frac{4}{s}$$

        $$Y(s)=\frac{s+4}{s(s+1)(s+2)}$$

        $$Y(s)=\frac{A}{s}+\frac{B}{s+1}+\frac{C}{s+2}$$

        \[\begin{cases}
            A=2
            \\
            B=-3
            \\
            C=1
        \end{cases}\]

        $$Y(s)=\frac{2}{s}+\frac{-3}{s+1}+\frac{1}{s+2}$$

        $$\mathcal{L}^{-1}\left\{Y(s)\right\}=y(t)=-3e^{-t}+e^{-2t}+2$$


% y'' + 3y' + 2y = t
    \item $y^{\prime \prime}+3y^{\prime}+2y=t$
        $$\mathcal{L}\left\{y^{\prime \prime}+3y^{\prime}+2y\right\}=\mathcal{L}\left\{t\right\}$$

        $$s^{2} Y(s) -s y(0) -y^{\prime}(0) +3s Y(s) - y(0) +2 Y(s)=\frac{1}{s^{2}}$$

        $$Y(s) \left( s^{2}+3s+2 \right)-1=\frac{1}{s^{2}}$$

        $$ Y(s)= \frac{s^{2}+1}{s^{2}(s+1)(s+2)}$$

        $$ Y(s)=\frac{A}{s^{2}}+\frac{B}{s}+\frac{C}{s+1}+\frac{D}{s+2}$$

        \[\begin{cases}
            A=\frac{1}{2}
            \\
            B=\frac{-3}{4}
            \\
            C=2
            \\
            D=\frac{-5}{4}
        \end{cases}\]

        $$ Y(s)=\frac{\frac{1}{2}}{s^{2}}+\frac{\frac{-3}{4}}{s}+\frac{2}{s+1}+
            \frac{\frac{-5}{4}}{s+2}$$

        $$\mathcal{L}^{-1}\left\{Y(s)\right\}=y(t)=2e^{-t}-\frac{5}{4}e^{-2t}+\frac{1}{2}t-
            \frac{3}{4}$$


% \newpage
% y'' + 3y' + 2y = sin(wt)
    \item $y^{\prime \prime}+3y^{\prime}+2y=sin(\omega t)$
        $$\mathcal{L}\left\{y^{\prime \prime}+3y^{\prime}+2y\right\}=
            \mathcal{L}\left\{sin(\omega t)\right\}$$

        $$Y(s)\left(s^{2}+3s+2\right)-1=\frac{\omega}{s^{2}+\omega^{2}}$$

        $$Y(s)=\frac{s^{2}+\omega^{2}+\omega}{(s^{2}+\omega^{2})(s+1)(s+2)}=\frac{A}{s+1}+
            \frac{B}{s+2}+\frac{Cs+D}{s^{2}+\omega^{2}}$$

        \[\begin{cases}
            A=\frac{\omega^{2}+\omega+1}{\omega^{2}+1}
            \\
            B=\frac{-\omega^{2}-\omega=4}{\omega^{2}+4}
            \\
            C=\frac{-3\omega}{\omega^{4}+5\omega^{2}+4}
            \\
            D=\frac{-\omega^{3}+2\omega}{\omega^{4}+5\omega^{2}+4}
        \end{cases}\]

        $$Y(s)=\frac{\frac{\omega^{2}+\omega+1}{\omega^{2}+1}}{s+1}+
            \frac{\frac{-\omega^{2}-\omega=4}{\omega^{2}+4}}{s+2}+
            \frac{\frac{-3\omega}{\omega^{4}+5\omega^{2}+4}s+
            \frac{-\omega^{3}+2\omega}{\omega^{4}+5\omega^{2}+4}}{s^{2}+\omega^{2}}$$

        $$\mathcal{L}^{-1}\left\{Y(s)\right\}=y(t)$$

        $$y(t)= \frac{\omega^{2}+\omega+1}{\omega^{2}+1}e^{-t} +
            \frac{-\omega^{2}-\omega-4}{\omega^{2}+4}e^{-2t}+
            \frac{1}{\omega^{4}+5\omega^{2}+4}\cdot \left[-3\omega cos(\omega t)+
            (-\omega^{2}+2)sin(\omega t)\right]$$


% y'' + 2y' + 2y = 0
    \item $y^{\prime \prime}+2y^{\prime}+2y=0$
        $$\mathcal{L}\left\{y^{\prime \prime}+2y^{\prime}+2y\right\}=\mathcal{L}\left\{0\right\}$$

        $$Y(s) \left(s^{2}+2s+2\right)-1=0$$

        $$Y(s)=\frac{1}{s^{2}+2s+2}=\frac{1}{(s+1)^{2}+1}$$

        $$\mathcal{L}^{-1}\left\{Y(s)\right\}=y(t)=e^{t}sin(t)$$

\newpage
% y'' + 2y' + 2y = 1
    \item $y^{\prime \prime}+2y^{\prime}+2y=1$
        $$\mathcal{L}\left\{y^{\prime \prime}+2y^{\prime}+2y\right\}=\mathcal{L}\left\{1\right\}$$

        $$Y(s)\left(s^{2}+2s+2\right)-1=\frac{1}{s} $$

        $$Y(s)=\frac{s+1}{s\left(s^{2}+2s+2\right)} =\frac{A}{s}+\frac{Bs+C}{s^{2}+2s+2}$$

        \[\begin{cases}
            A=\frac{1}{2}
            \\
            B=\frac{-1}{2}
            \\
            C=0
        \end{cases}\]

        $$ Y(s)=\frac{1}{2s}+\frac{\frac{1}{2}s-1+1}{s^{2}+2s+2}$$

        $$\mathcal{L}^{-1}\left\{Y(s)\right\}=y(t)=\frac{1}{2}
            \left(1-e^{-t}\left[cos(t)-sin(t)\right]\right) $$


\end{itemize}
\end{document}
